Hierarchy is now properly passed to eval from brand model, custom correctness proof of NRAEnv to ImpEJson
Signed-off-by: Jerome Simeon <jeromesimeon@me.com>

compiler/lib/config.ml
@@ -133,7 +133,6 @@ let complete_configuration gconf =
 (* Driver config *)
 
 let driver_conf_of_global_conf gconf qname cname =
-  let brand_rel = Type_util.brand_relation_of_brand_model gconf.gconf_schema.Type_util.sch_brand_model in
   let qcname =
     begin match cname with
     | None -> None
@@ -144,7 +143,6 @@ let driver_conf_of_global_conf gconf qname cname =
   { Compiler.comp_qname = char_list_of_string qname;
     Compiler.comp_qname_lowercase = char_list_of_string (String.lowercase_ascii (gconf.gconf_prefix ^ qname));
     comp_class_name = qcname;
-    comp_brand_rel = brand_rel;
     comp_mr_vinit = char_list_of_string gconf.gconf_mr_vinit;
     comp_constants = constants_config;
     comp_java_imports = char_list_of_string gconf.gconf_java_imports;
