compiler/src/Compiler/Lib/QEval.v
@@ -23,61 +23,61 @@ Require Import CompEval.
 Module QEval(runtime:CompilerRuntime).
 
   Section QE.
-  Context {h:list(string*string)}.
+    Context {bm:brand_model}.
 
-  (* Inputs to eval *)
-  Definition constant_env : Set := list (string*data).
-  Definition dconstant_env : Set := list (string*ddata).
-  Definition world_env : Set := list data.
+    (* Inputs to eval *)
+    Definition constant_env : Set := list (string*data).
+    Definition dconstant_env : Set := list (string*ddata).
+    Definition world_env : Set := list data.
   
-  (* Eval for arbitrary (local) constant environments *)
-  Definition eval_camp_rule : camp_rule -> constant_env -> option data := @eval_camp_rule _ h.
-  Definition eval_camp_rule_debug : bool -> camp_rule -> constant_env -> string := @eval_camp_rule_debug _ h.
+    (* Eval for arbitrary (local) constant environments *)
+    Definition eval_camp_rule : camp_rule -> constant_env -> option data := @eval_camp_rule _ _ bm.
+    Definition eval_camp_rule_debug : bool -> camp_rule -> constant_env -> string := @eval_camp_rule_debug _ _ bm.
   
-  Definition eval_camp : camp -> constant_env -> option data := @eval_camp _ h.
-  Definition eval_camp_debug : bool -> camp -> constant_env -> string := @eval_camp_debug _ h.
+    Definition eval_camp : camp -> constant_env -> option data := @eval_camp _ _ bm.
+    Definition eval_camp_debug : bool -> camp -> constant_env -> string := @eval_camp_debug _ _ bm.
 
-  Definition eval_oql : oql -> constant_env -> option data := @eval_oql _ h.
-  Definition eval_lambda_nra : lambda_nra -> constant_env -> option data := @eval_lambda_nra _ h.
+    Definition eval_oql : oql -> constant_env -> option data := @eval_oql _ _ bm.
+    Definition eval_lambda_nra : lambda_nra -> constant_env -> option data := @eval_lambda_nra _ _ bm.
 
-  Definition eval_nra : nra -> constant_env -> option data := @eval_nra _ h.
-  Definition eval_nraenv_core : nraenv_core -> constant_env -> option data := @eval_nraenv_core _ h.
-  Definition eval_nraenv : nraenv -> constant_env -> option data := @eval_nraenv _ h.
+    Definition eval_nra : nra -> constant_env -> option data := @eval_nra _ _ bm.
+    Definition eval_nraenv_core : nraenv_core -> constant_env -> option data := @eval_nraenv_core _ _ bm.
+    Definition eval_nraenv : nraenv -> constant_env -> option data := @eval_nraenv _ _ bm.
 
-  Definition eval_nnrc : nnrc -> constant_env -> option data := @eval_nnrc _ h.
+    Definition eval_nnrc : nnrc -> constant_env -> option data := @eval_nnrc _ _ bm.
 
-  Definition eval_nnrs : nnrs -> constant_env -> option data := @eval_nnrs _ h.
+    Definition eval_nnrs : nnrs -> constant_env -> option data := @eval_nnrs _ _ bm.
 
-  Definition eval_nnrcmr : nnrcmr -> dconstant_env -> option data := @eval_nnrcmr _ _ h.
-  Definition eval_dnnrc {bm:brand_model} : dnnrc -> dconstant_env -> option data := @eval_dnnrc _ _ h.
+    Definition eval_nnrcmr : nnrcmr -> dconstant_env -> option data := @eval_nnrcmr _ _ _ bm.
+    Definition eval_dnnrc {bm:brand_model} : dnnrc -> dconstant_env -> option data := @eval_dnnrc _ _ bm.
 
-  (* Eval driver *)
+    (* Eval driver *)
 
-  Definition eval_input : Set := eval_input.
-  Definition eval_output : Set := eval_output.
+    Definition eval_input : Set := eval_input.
+    Definition eval_output : Set := eval_output.
 
-  Definition eval_query {bm:brand_model} : query -> eval_input -> eval_output := @eval_query _ _ _ _ _ bm h.
+    Definition eval_query {bm:brand_model} : query -> eval_input -> eval_output := @eval_query _ _ _ _ _ bm.
 
-  Definition eval_query_debug {bm:brand_model} : query -> eval_input -> eval_output := @eval_query_debug _ _ _ _ _ _ h.
+    Definition eval_query_debug {bm:brand_model} : query -> eval_input -> eval_output := @eval_query_debug _ _ _ _ _ bm.
 
-  (* Eval for single 'world' collection *)
-  Definition eval_camp_rule_world : camp_rule -> world_env -> option data := @eval_camp_rule_world _ h.
-  Definition eval_camp_rule_world_debug : bool -> camp_rule -> world_env -> string := @eval_camp_rule_world_debug _ h.
+    (* Eval for single 'world' collection *)
+    Definition eval_camp_rule_world : camp_rule -> world_env -> option data := @eval_camp_rule_world _ _ bm.
+    Definition eval_camp_rule_world_debug : bool -> camp_rule -> world_env -> string := @eval_camp_rule_world_debug _ _ bm.
   
-  Definition eval_camp_world : camp -> world_env -> option data := @eval_camp_world _ h.
-  Definition eval_camp_world_debug : bool -> camp -> world_env -> string := @eval_camp_world_debug _ h.
+    Definition eval_camp_world : camp -> world_env -> option data := @eval_camp_world _ _ bm.
+    Definition eval_camp_world_debug : bool -> camp -> world_env -> string := @eval_camp_world_debug _ _ bm.
 
-  Definition eval_oql_world : oql -> world_env -> option data := @eval_oql_world _ h.
-  Definition eval_lambda_nra_world : lambda_nra -> world_env -> option data := @eval_lambda_nra_world _ h.
+    Definition eval_oql_world : oql -> world_env -> option data := @eval_oql_world _ _ bm.
+    Definition eval_lambda_nra_world : lambda_nra -> world_env -> option data := @eval_lambda_nra_world _ _ bm.
 
-  Definition eval_nra_world : nra -> world_env -> option data := @eval_nra_world _ h.
-  Definition eval_nraenv_core_world : nraenv_core -> world_env -> option data := @eval_nraenv_core_world _ h.
-  Definition eval_nraenv_world : nraenv -> world_env -> option data := @eval_nraenv_world _ h.
+    Definition eval_nra_world : nra -> world_env -> option data := @eval_nra_world _ _ bm.
+    Definition eval_nraenv_core_world : nraenv_core -> world_env -> option data := @eval_nraenv_core_world _ _ bm.
+    Definition eval_nraenv_world : nraenv -> world_env -> option data := @eval_nraenv_world _ _ bm.
 
-  Definition eval_nnrc_world : nnrc -> world_env -> option data := @eval_nnrc_world _ h.
+    Definition eval_nnrc_world : nnrc -> world_env -> option data := @eval_nnrc_world _ _ bm.
 
-  Definition eval_nnrcmr_world : nnrcmr -> world_env -> option data := @eval_nnrcmr_world _ _ h.
-  Definition eval_dnnrc_world {bm:brand_model} : dnnrc -> world_env -> option data := @eval_dnnrc_world _ _ h.
+    Definition eval_nnrcmr_world : nnrcmr -> world_env -> option data := @eval_nnrcmr_world _ _ _ bm.
+    Definition eval_dnnrc_world {bm:brand_model} : dnnrc -> world_env -> option data := @eval_dnnrc_world _ _ bm.
   End QE.
 
 End QEval.
