compiler/src/Compiler/Enhanced/EnhancedTypeToJSON.v
@@ -17,7 +17,6 @@ Require Import ZArith.
 Require Import EquivDec.
 Require Import RelationClasses.
 Require Import Equivalence.
-Require Import ToString.
 Require Import String.
 Require Import Utils.
 Require Import JSONSystem.
